Simpler Impl.header_encrypt with functional correctness

src/QUIC.Impl.Header.fst
@@ -104,8 +104,7 @@ let block_of_sample (a: Spec.Agile.Cipher.cipher_alg)
 
 (* A more careful version of header_encrypt wrt. constant-time issues, which does not test or truncate on pn_len *)
 
-inline_for_extraction
-let pn_sizemask_ct (pn_len:nat { pn_len < 4 }) : lbytes 4 =
+let pn_sizemask_ct (pn_len:nat { pn_len < 4 }) : Tot (lbytes 4) =
   let open FStar.Endianness in
   FStar.Math.Lemmas.pow2_lt_compat 32 (24 - (8 `op_Multiply` pn_len));
   FStar.Endianness.n_to_be 4 (pow2 32 - pow2 (24 - (8 `op_Multiply` pn_len)))
@@ -244,115 +243,97 @@ let secret_xor_inplace_eq
 let header_encrypt_ct_secret_preserving_not_retry_spec
   (a:ea)
   (hpk: Spec.Agile.Cipher.key (Spec.Agile.AEAD.cipher_alg_of_supported_alg a))
-  (is_short: bool)
-  (pn_len: PN.packet_number_length_t)
-  (f: Secret.uint8)
-  (pn_and_c: Seq.seq Secret.uint8 { Seq.length pn_and_c >= 20 })
-: GTot (Secret.uint8 & Seq.seq Secret.uint8)
-= let sample = Seq.slice pn_and_c 4 20 in
-  let mask = Spec.block_of_sample (Spec.Agile.AEAD.cipher_alg_of_supported_alg a) hpk sample in
-  let pnmask = secret_and_inplace (Seq.slice mask 1 5) (Seq.seq_hide (pn_sizemask_ct (Secret.v pn_len - 1))) 0 in
-  let protected_bits = if is_short then 5ul else 4ul in
+  (h: Spec.header { ~ (Spec.is_retry h) })
+  (r: Seq.seq Secret.uint8 {
+    Seq.length r >= ParseSpec.pn_offset h + 20
+  })
+: GTot (Seq.seq Secret.uint8)
+= 
+  let pn_offset = ParseSpec.pn_offset h in
+  let pn_len = Secret.v (Spec.pn_length h) - 1 in
+  let sample = (Seq.slice r (pn_offset + 4) (pn_offset + 20)) in
+  let mask = (Spec.block_of_sample (Spec.Agile.AEAD.cipher_alg_of_supported_alg a) hpk sample) in
+  let pnmask = secret_and_inplace (Seq.slice mask 1 5) (Seq.seq_hide (pn_sizemask_ct pn_len)) 0 in
+  let f = Seq.index r 0 in
+  let protected_bits = if Spec.MShort? h then 5ul else 4ul in
   let f' = Secret.set_bitfield f 0ul protected_bits (Secret.get_bitfield (f `Secret.logxor` Seq.index mask 0) 0ul protected_bits) in
-  let pn_and_c' = secret_xor_inplace pn_and_c pnmask 0 in
-  f', pn_and_c'
+  let r = secret_xor_inplace r pnmask pn_offset in
+  let r = Seq.cons f' (Seq.slice r 1 (Seq.length r)) in
+  r
+
+#push-options "--z3rlimit 256 --query_stats --z3cliopt smt.arith.nl=false --fuel 2 --ifuel 2"
+
+#restart-solver
 
 let header_encrypt_ct_secret_preserving_not_retry_spec_correct
   (a:ea)
   (hpk: Spec.Agile.Cipher.key (Spec.Agile.AEAD.cipher_alg_of_supported_alg a))
   (h: Spec.header)
   (c: cbytes)
-  (f: Secret.uint8)
-  (pub: Seq.seq U8.t)
-  (pn_and_c: Seq.seq Secret.uint8)
 : Lemma
   (requires (
-    (~ (Spec.is_retry h)) /\
-    (ParseSpec.format_header h `Seq.append` c) `Seq.equal` (Secret.reveal f `Seq.cons` (pub `Seq.append` Seq.seq_reveal pn_and_c)) /\
-    1 + Seq.length pub == ParseSpec.pn_offset h
+    (~ (Spec.is_retry h))
   ))
   (ensures (
-    Seq.length pn_and_c >= 20 /\ (
-    let (f', pn_and_c') = header_encrypt_ct_secret_preserving_not_retry_spec a hpk (Spec.MShort? h) (ParseSpec.pn_length h) f pn_and_c in
-    Spec.header_encrypt a hpk h c `Seq.equal` (Secret.reveal f' `Seq.cons` (pub `Seq.append` Seq.seq_reveal pn_and_c'))
-  )))
-=
-(*
-  let pn_length = Secret.v (ParseSpec.pn_length h) in
-  let pn_len_1 = pn_length - 1 in
-  assert (ParseSpec.pn_offset h + pn_length == Seq.length (ParseSpec.format_header h));
-  let s = ParseSpec.format_header h `Seq.append` c in
-  let t = Secret.reveal f `Seq.cons` (pub `Seq.append` Seq.seq_reveal pn_and_c) in
-  assert (Seq.length (ParseSpec.format_header h `Seq.append` c) == Seq.length (Secret.reveal f `Seq.cons` (pub `Seq.append` Seq.seq_reveal pn_and_c)));
-  assert (1 + (Seq.length pub + Seq.length pn_and_c) == Seq.length (ParseSpec.format_header h) + Seq.length c);
-  assert (Seq.length pn_and_c == pn_length + Seq.length c);
-  assert (pn_length + Seq.length c >= 20);
-  Seq.slice_slice s 0 (Seq.length (ParseSpec.format_header h)) 0 (1 + Seq.length pub);
-  Seq.slice_slice t 0 (1 + Seq.length pub) 4 20;
-  assert (Seq.slice (Seq.seq_reveal pn_and_c) 4 20 `Seq.equal` Seq.slice s (3 - pn_len_1) (19 - pn_len_1));
-*)
-  admit ()
-
-unfold
-let header_encrypt_ct_secret_preserving_not_retry_spec_post
-  (a:ea)
-  (hpk: Ghost.erased (Spec.Agile.Cipher.key (Spec.Agile.AEAD.cipher_alg_of_supported_alg a)))
-  (is_short: bool)
-  (pn_len: PN.packet_number_length_t)
-  (f: Ghost.erased Secret.uint8)
-  (pub: Ghost.erased (Seq.seq U8.t))
-  (pn_and_c: Ghost.erased (Seq.seq Secret.uint8))
-  (f' : Ghost.erased Secret.uint8)
-  (pub' : Ghost.erased (Seq.seq U8.t))
-  (pn_and_c' : Ghost.erased (Seq.seq Secret.uint8))
-: Tot Type0
-= 
-  Seq.length pn_and_c >= 20 /\ (
-  let (f_, pn_and_c_) =
-      header_encrypt_ct_secret_preserving_not_retry_spec a hpk is_short pn_len f pn_and_c
-  in
-  f_ == Ghost.reveal f' /\
-  Ghost.reveal pub `Seq.equal` Ghost.reveal pub' /\
-  pn_and_c_ `Seq.equal` Ghost.reveal pn_and_c'
-  )
-
-let header_encrypt_ct_secret_preserving_not_retry_spec_correct'
-  (a:ea)
-  (hpk: Ghost.erased (Spec.Agile.Cipher.key (Spec.Agile.AEAD.cipher_alg_of_supported_alg a)))
-  (h: Ghost.erased Spec.header)
-  (is_short: bool)
-  (pn_len: PN.packet_number_length_t)
-  (c: Ghost.erased cbytes)
-  (f: Ghost.erased Secret.uint8)
-  (pub: Ghost.erased (Seq.seq U8.t))
-  (pn_and_c: Ghost.erased (Seq.seq Secret.uint8))
-  (req: squash (
-    (~ (Spec.is_retry h)) /\
-    is_short == (Spec.MShort? h) /\
-    pn_len == (Spec.pn_length h) /\
-    (ParseSpec.format_header h `Seq.append` c) `Seq.equal` (Secret.reveal f `Seq.cons` (pub `Seq.append` Seq.seq_reveal pn_and_c)) /\
-    1 + Seq.length pub == ParseSpec.pn_offset h
+    let r = ParseSpec.format_header h `Seq.append` c in
+    Seq.length r >= ParseSpec.pn_offset h + 20 /\
+    Spec.header_encrypt a hpk h c == Seq.seq_reveal (header_encrypt_ct_secret_preserving_not_retry_spec a hpk h (Seq.seq_hide r))
   ))
-: Tot (
-    x: squash (Seq.length pn_and_c >= 20) & (
-    (f' : Secret.uint8) ->
-    (pub' : Seq.seq U8.t) ->
-    (pn_and_c' : Seq.seq Secret.uint8) ->
-    Lemma
-      (requires (
-        header_encrypt_ct_secret_preserving_not_retry_spec_post a hpk is_short pn_len f pub pn_and_c f' pub' pn_and_c'
-      ))
-      (ensures (
-        Spec.header_encrypt a hpk h c == (Secret.reveal f' `Seq.cons` (pub' `Seq.append` Seq.seq_reveal pn_and_c'))
-      ))
-  ))
-= header_encrypt_ct_secret_preserving_not_retry_spec_correct a hpk h c f pub pn_and_c;
-  (| (), (fun _ _ pn_and_c' ->
-    let (f_, pn_and_c_) =
-      header_encrypt_ct_secret_preserving_not_retry_spec a hpk (Spec.MShort? h) (ParseSpec.pn_length h) f pn_and_c
-    in
-    ()
-  ) |)
+= header_encrypt_ct_correct a hpk h c;
+  let fmt = ParseSpec.format_header h in
+  let len = Seq.length fmt in
+  let pr = fmt `Seq.append` c in
+  assert (Seq.length pr >= ParseSpec.pn_offset h + 20);
+  let pn_len = Secret.v (Spec.pn_length h) - 1 in
+  let psample = Seq.slice c (3 - pn_len) (19 - pn_len) in
+  assert (c `Seq.equal` Seq.slice pr len (Seq.length pr));
+  let pn_off = ParseSpec.pn_offset h in
+  assert (pn_off + pn_len + 1 == len);
+  assert (c == Seq.slice pr (pn_off + pn_len + 1) (Seq.length pr));
+  Seq.slice_slice pr (pn_off + pn_len + 1) (Seq.length pr) (3 - pn_len) (19 - pn_len);
+  assert (psample == Seq.slice pr (pn_off + 4) (pn_off + 20));
+  let r = Seq.seq_hide #Secret.U8 pr in
+  let sample = Seq.slice r (pn_off + 4) (pn_off + 20) in
+  assert (sample == Seq.seq_hide #Secret.U8 psample);
+  let mask = Spec.block_of_sample (Spec.Agile.AEAD.cipher_alg_of_supported_alg a) hpk sample in
+  let pmask = Seq.seq_reveal mask in
+  assert (mask == Seq.seq_hide pmask);
+  let mask15 = Seq.slice mask 1 5 in
+  let ppnszmask = pn_sizemask_ct pn_len in
+  let pnszmask = Seq.seq_hide ppnszmask in
+  let pnmask = secret_and_inplace mask15 pnszmask 0 in
+  let pmask15 = Seq.slice pmask 1 5 in
+  let ppnmask = Lemmas.and_inplace pmask15 ppnszmask 0 in
+  secret_and_inplace_eq mask15 pnszmask 0;
+  assert (pnmask == Seq.seq_hide #Secret.U8 ppnmask);
+  let f = Seq.index r 0 in
+  let pf : Secret.uint_t Secret.U8 Secret.PUB = Seq.index pr 0 in
+  assert (f == Secret.hide #Secret.U8 #Secret.PUB pf);
+  let protected_bits = if Spec.MShort? h then 5ul else 4ul in
+  let pf' = U8.uint_to_t (BF.set_bitfield (U8.v pf) 0 (U32.v protected_bits) (BF.get_bitfield (U8.v pf `FStar.UInt.logxor` U8.v (Seq.index pmask 0)) 0 (U32.v protected_bits))) in
+  let f' = Secret.set_bitfield f 0ul protected_bits (Secret.get_bitfield (f `Secret.logxor` Seq.index mask 0) 0ul protected_bits) in
+  assert (U8.v pf' == Secret.v f');
+  assert (f' == Secret.hide #Secret.U8 pf');
+  let pr1 = Lemmas.xor_inplace pr ppnmask pn_off in
+  let r1 = secret_xor_inplace r pnmask pn_off in
+  secret_xor_inplace_eq r pnmask pn_off;
+  assert (r1 == Seq.seq_hide #Secret.U8 pr1);
+  let r2 = Seq.cons f' (Seq.slice r1 1 (Seq.length r1)) in
+  let pr2 = Seq.cons pf' (Seq.slice pr1 1 (Seq.length pr1)) in
+  Seq.cons_seq_hide #Secret.U8 pf' (Seq.slice pr1 1 (Seq.length pr1));
+  assert (r2 == Seq.seq_hide #Secret.U8 pr2)
+
+#pop-options
+
+inline_for_extraction
+noextract
+let pn_sizemask (dst: B.buffer Secret.uint8) (pn_len: PN.packet_number_length_t): HST.Stack unit
+  (requires fun h0 ->
+    B.live h0 dst /\ B.length dst == 4)
+  (ensures fun h0 _ h1 ->
+    B.as_seq h1 dst `Seq.equal` Seq.seq_hide (pn_sizemask_ct (Secret.v pn_len - 1)) /\
+    B.(modifies (loc_buffer dst) h0 h1))
+= admit ()
 
 #push-options "--z3rlimit 200"
 inline_for_extraction noextract
@@ -464,32 +445,6 @@ let op_inplace
       Seq.slice (B.as_seq h1 dst) (U32.v (ofs `U32.add` src_len)) (B.length dst))
 = op_inplace' dst (B.len dst) src src_len ofs op
 
-inline_for_extraction
-noextract
-let pn_sizemask (dst: B.buffer Secret.uint8) (pn_len: PN.packet_number_length_t): HST.Stack unit
-  (requires fun h0 ->
-    B.live h0 dst /\ B.length dst == 4)
-  (ensures fun h0 _ h1 ->
-    B.as_seq h1 dst `Seq.equal` Seq.seq_hide (pn_sizemask_ct (Secret.v pn_len - 1)) /\
-    B.(modifies (loc_buffer dst) h0 h1))
-= admit ()
-
-(*
-let open FStar.Mul in
-  [@ inline_let ]
-  let pn_len32 = FStar.Int.Cast.uint8_to_uint32 pn_len in
-  assert (U32.v pn_len32 = U8.v pn_len);
-  assert_norm (0xffffffff = pow2 32 - 1);
-  assert (24 - 8 * U32.v pn_len32 < 32);
-  assert (24 - 8 * U32.v pn_len32 >= 0);
-  FStar.UInt.shift_left_value_lemma #32 1 (24 - 8 * U32.v pn_len32);
-  FStar.Math.Lemmas.pow2_lt_compat 32 (24 - 8 * U32.v pn_len32);
-  FStar.Math.Lemmas.modulo_lemma (pow2 (24 - 8 * U32.v pn_len32)) (pow2 32);
-  assert (U32.(v (1ul <<^ (24ul -^ 8ul *^ pn_len32))) = pow2 (24 - 8 * U32.v pn_len32));
-  LowStar.Endianness.store32_be dst
-    U32.(0xfffffffful -^ (1ul <<^ (24ul -^ 8ul *^ pn_len32)) +^ 1ul)
-*)
-
 #push-options "--z3rlimit 512 --query_stats --z3cliopt smt.arith.nl=false --fuel 2 --ifuel 1"
 
 #restart-solver
@@ -498,28 +453,35 @@ let header_encrypt_ct_secret_preserving_not_retry
   (a: ea)
   (s: CTR.state (Spec.Agile.AEAD.cipher_alg_of_supported_alg a))
   (k: B.buffer Secret.uint8)
+  (h: Ghost.erased Spec.header)
   (is_short: bool)
+  (pn_offset: U32.t)
   (pn_len: PN.packet_number_length_t)
-  (f: B.buffer Secret.uint8)
-  (pub: B.buffer Secret.uint8)
-  (pn_and_c: B.buffer Secret.uint8)
+  (dst: B.buffer Secret.uint8)
 : HST.Stack unit
   (requires (fun m ->
-    B.all_live m [B.buf k; B.buf f; B.buf pub; B.buf pn_and_c] /\
+    let fmt = (Parse.format_header h) in
+    let hlen = Seq.length fmt in
+    B.all_live m [B.buf k; B.buf dst] /\
     CTR.invariant m s /\
     B.all_disjoint
-      [ CTR.footprint m s; B.loc_buffer k; B.loc_buffer f; B.loc_buffer pub; B.loc_buffer pn_and_c] /\
+      [ CTR.footprint m s; B.loc_buffer k; B.loc_buffer dst] /\
     B.length k == Spec.Agile.Cipher.key_length (Spec.Agile.AEAD.cipher_alg_of_supported_alg a) /\
-    B.length f == 1 /\
-    B.length pn_and_c >= 20
+    (~ (Spec.is_retry h)) /\
+    is_short == (Spec.MShort? h) /\
+    U32.v pn_offset == Parse.pn_offset h /\
+    pn_len == Parse.pn_length h /\
+    hlen + 19 <= B.length dst /\
+    Seq.slice (Seq.seq_reveal #Secret.U8 (B.as_seq m dst)) 0 hlen == fmt
   ))
   (ensures (fun m _ m' ->
-    B.modifies (B.loc_buffer f `B.loc_union` B.loc_buffer pn_and_c `B.loc_union` CTR.footprint m s) m m' /\
+    B.modifies (B.loc_buffer dst `B.loc_union` CTR.footprint m s) m m' /\
     CTR.invariant m' s /\
     CTR.footprint m s == CTR.footprint m' s /\
-    header_encrypt_ct_secret_preserving_not_retry_spec_post a (B.as_seq m k) is_short pn_len (Seq.index (B.as_seq m f) 0) (Seq.seq_reveal (B.as_seq m pub)) (B.as_seq m pn_and_c) (Seq.index (B.as_seq m' f) 0) (Seq.seq_reveal (B.as_seq m' pub)) (B.as_seq m' pn_and_c)
+    header_encrypt_ct_secret_preserving_not_retry_spec a (B.as_seq m k) h (B.as_seq m dst) == B.as_seq m' dst
   ))
-= let m0 = HST.get () in
+= assert (U32.v pn_offset + 20 <= B.length dst);
+  let m0 = HST.get () in
   HST.push_frame ();
   let m01 = HST.get () in
   let mask = B.alloca (Secret.to_u8 0uy) 16ul in
@@ -530,10 +492,10 @@ let header_encrypt_ct_secret_preserving_not_retry
   let m03 = HST.get () in
   assert (B.loc_disjoint (B.loc_buffer mask) (B.loc_buffer pn_sm));
   assert (CTR.footprint m03 s == CTR.footprint m0 s);
-  assert (B.loc_disjoint (B.loc_buffer mask `B.loc_union` B.loc_buffer pn_sm) (CTR.footprint m0 s `B.loc_union` B.loc_buffer k `B.loc_union` B.loc_buffer f `B.loc_union` B.loc_buffer pub `B.loc_union` B.loc_buffer pn_and_c));
-  let sample = B.sub pn_and_c 4ul 16ul in
+  assert (B.loc_disjoint (B.loc_buffer mask `B.loc_union` B.loc_buffer pn_sm) (CTR.footprint m0 s `B.loc_union` B.loc_buffer k `B.loc_union` B.loc_buffer dst));
+  let sample = B.sub dst (pn_offset `U32.add` 4ul) 16ul in
   let m1 = HST.get () in
-  let gsample = Ghost.hide (Seq.slice (B.as_seq m0 pn_and_c) 4 20) in
+  let gsample = Ghost.hide (Seq.slice (B.as_seq m0 dst) (U32.v pn_offset + 4) (U32.v pn_offset + 20)) in
   assert (B.as_seq m1 sample == Ghost.reveal gsample);
   block_of_sample (Spec.Agile.AEAD.cipher_alg_of_supported_alg a) mask s k sample;
   let m2 = HST.get () in
@@ -553,15 +515,33 @@ let header_encrypt_ct_secret_preserving_not_retry
   let mask_0 = B.index mask 0ul in
   assert (mask_0 == Seq.index (B.as_seq m4 (B.gsub mask 0ul 1ul)) 0);
   assert (mask_0 == Seq.index gmask 0);
-  let f_ = B.index f 0ul in
-  assert (f_ == Seq.index (B.as_seq m0 f) 0);
+  let f_ = B.index dst 0ul in
+  assert (f_ == Seq.index (B.as_seq m0 dst) 0);
   let f' = Secret.set_bitfield f_ 0ul protected_bits (Secret.get_bitfield (f_ `Secret.logxor` mask_0) 0ul protected_bits) in
-  B.upd f 0ul f' ;
-  op_inplace pn_and_c pnmask 4ul 0ul (Secret.logxor #Secret.U8 #Secret.SEC);
-  HST.pop_frame ();
+  op_inplace dst pnmask 4ul pn_offset (Secret.logxor #Secret.U8 #Secret.SEC);
   let m5 = HST.get () in
-  assert (f' == Seq.index (B.as_seq m5 f) 0);
-  assert (B.as_seq m5 pn_and_c == secret_xor_inplace (B.as_seq m0 pn_and_c) gpnmask 0)
+  let gr1 = Ghost.hide (secret_xor_inplace (B.as_seq m0 dst) gpnmask (U32.v pn_offset)) in
+  assert (B.as_seq m5 dst == Ghost.reveal gr1);
+  B.upd dst 0ul f' ;
+  HST.pop_frame ();
+  let m6 = HST.get () in
+  assert (B.as_seq m6 dst `Seq.equal` (f' `Seq.cons` Seq.slice (Ghost.reveal gr1) 1 (B.length dst)))
+
+(*
+let open FStar.Mul in
+  [@ inline_let ]
+  let pn_len32 = FStar.Int.Cast.uint8_to_uint32 pn_len in
+  assert (U32.v pn_len32 = U8.v pn_len);
+  assert_norm (0xffffffff = pow2 32 - 1);
+  assert (24 - 8 * U32.v pn_len32 < 32);
+  assert (24 - 8 * U32.v pn_len32 >= 0);
+  FStar.UInt.shift_left_value_lemma #32 1 (24 - 8 * U32.v pn_len32);
+  FStar.Math.Lemmas.pow2_lt_compat 32 (24 - 8 * U32.v pn_len32);
+  FStar.Math.Lemmas.modulo_lemma (pow2 (24 - 8 * U32.v pn_len32)) (pow2 32);
+  assert (U32.(v (1ul <<^ (24ul -^ 8ul *^ pn_len32))) = pow2 (24 - 8 * U32.v pn_len32));
+  LowStar.Endianness.store32_be dst
+    U32.(0xfffffffful -^ (1ul <<^ (24ul -^ 8ul *^ pn_len32)) +^ 1ul)
+*)
 
 #restart-solver
 
@@ -572,29 +552,15 @@ let header_encrypt
   else begin
     let m = HST.get () in
     let hpk = Ghost.hide (B.as_seq m k) in
-    let cipher = Ghost.hide (Seq.slice (B.as_seq m dst) (Seq.length (ParseSpec.format_header (G.reveal h))) (B.length dst)) in
-    let f = Ghost.hide (Secret.hide #Secret.U8 (Seq.index (B.as_seq m dst) 0)) in
-    let pub = Ghost.hide (Seq.slice (B.as_seq m dst) 1 (U32.v public_len)) in
-    let pn_and_cipher = Ghost.hide (Seq.slice (Seq.seq_hide #Secret.U8 (B.as_seq m dst)) (U32.v public_len) (B.length dst)) in
-    let (| prf, phi |) = header_encrypt_ct_secret_preserving_not_retry_spec_correct'
-        a
-        hpk
-        h
-        is_short
-        pn_len
-        cipher
-        f
-        pub
-        pn_and_cipher
-        ()
-    in
+    let fmt = Ghost.hide (ParseSpec.format_header (G.reveal h)) in
+    let cipher = Ghost.hide (Seq.slice (B.as_seq m dst) (Seq.length fmt)  (B.length dst)) in
+    assert (B.as_seq m dst `Seq.equal` (fmt `Seq.append` cipher));
+    header_encrypt_ct_secret_preserving_not_retry_spec_correct a hpk h cipher;
+    assert (U32.v public_len + 20 <= B.length dst);
     let post (cont: Seq.lseq Secret.uint8 (B.length dst)) (m1: HS.mem) : GTot Type0 =
-        let f' = Seq.index cont 0 in
-        let pub' = Seq.seq_reveal #Secret.U8 (Seq.slice cont 1 (U32.v public_len)) in 
-        let pn_and_c' = Seq.slice cont (U32.v public_len) (B.length dst) in
-        header_encrypt_ct_secret_preserving_not_retry_spec_post a hpk is_short pn_len f pub pn_and_cipher f' pub' pn_and_c' /\
-        CTR.invariant m1 s /\
-        CTR.footprint m1 s == CTR.footprint m s
+      header_encrypt_ct_secret_preserving_not_retry_spec a hpk h (Seq.seq_hide (B.as_seq m dst)) == cont /\
+      CTR.invariant m1 s /\
+      CTR.footprint m1 s == CTR.footprint m s
     in
     SecretBuffer.with_whole_buffer_hide_weak_modifies'
       #unit
@@ -607,31 +573,12 @@ let header_encrypt
         post cont m1
       )
       (fun _ bs ->
-        let bf = B.sub bs 0ul 1ul in
-        let bpub = B.sub bs 1ul (public_len `U32.sub` 1ul) in
-        let bpn_and_c = B.offset bs public_len in
-        let m1 = HST.get () in
-        assert (Seq.index (B.as_seq m1 bf) 0 == Ghost.reveal f);
-        assert (Seq.seq_reveal (B.as_seq m1 bpub) `Seq.equal` Ghost.reveal pub);
-        assert (B.as_seq m1 bpn_and_c == Ghost.reveal pn_and_cipher);
-        header_encrypt_ct_secret_preserving_not_retry a s k is_short pn_len bf bpub bpn_and_c
+        header_encrypt_ct_secret_preserving_not_retry a s k h is_short public_len pn_len bs
       )
-      ;
-      let m' = HST.get () in
-      let cont_p = Ghost.hide (B.as_seq m' dst) in
-      let cont_s = Ghost.hide (Seq.seq_hide #Secret.U8 cont_p) in
-      assert (post cont_s m');
-      let f' = Ghost.hide (Seq.index cont_s 0) in
-      let pub' = Ghost.hide (Seq.seq_reveal #Secret.U8 (Seq.slice cont_s 1 (U32.v public_len))) in
-      let pn_and_cipher' = Ghost.hide (Seq.slice cont_s (U32.v public_len) (B.length dst)) in
-      assert (
-        header_encrypt_ct_secret_preserving_not_retry_spec_post a hpk is_short pn_len f pub pn_and_cipher f' pub' pn_and_cipher'
-      );
-      assert (
-        cont_p `Seq.equal` (Secret.reveal f' `Seq.cons` (pub' `Seq.append` Seq.seq_reveal pn_and_cipher'))
-      );
-      phi f' pub' pn_and_cipher' ;
-      assert (header_encrypt_post a s k dst h is_short is_retry public_len pn_len m m') // by (FStar.Tactics.fail "abc")
+    ;
+    let m' = HST.get () in
+    assert (B.as_seq m' dst == Seq.seq_reveal (header_encrypt_ct_secret_preserving_not_retry_spec a hpk h (Seq.seq_hide (B.as_seq m dst))));
+    assert (B.as_seq m' dst == Spec.header_encrypt a (B.as_seq m k) h cipher)
   end
 
 #pop-options
